src/Refinement/ProgLang/Hoare.v
@@ -113,7 +113,7 @@ Proof.
     end.
   - inv_exec.
     + (* p crashed before running *)
-      assert (exec p w' (Crashed w')) as Hexec by constructor.
+      assert (exec p w' (Crashed w')) as Hexec by ( constructor; eauto ).
       eapply RExecCrash in Hexec; eauto.
       eapply H0 in H2; repeat deex.
       eapply H in Hexec; simpl in *; safe_intuition (repeat deex; eauto).
