src/Refinement/ProgLang/NoCrashes.v
@@ -1,0 +1,34 @@
+Require Import ProgLang.Prog.
+Require Import ProgLang.Hoare.
+
+Axiom cannot_crash : can_crash = False.
+
+Ltac cannot_crash' :=
+  exfalso;
+  match goal with
+  | H: can_crash |- _ => rewrite cannot_crash in H; exact H
+  end.
+
+Theorem exec_cannot_crash : forall T (p : prog T) w w',
+  exec p w (Crashed w') -> False.
+Proof.
+  intros.
+  remember (Crashed w') as cw.
+  induction H; try congruence; cannot_crash'.
+Qed.
+
+Theorem always_rec_noop : forall R State rec_impl abstr effect,
+  rec_noop (R := R) (State := State) rec_impl abstr effect.
+Proof.
+  unfold rec_noop; simpl; intros.
+  unfold prog_spec; simpl; intros.
+  inv_rexec; inv_ret; eauto.
+  cannot_crash'.
+Qed.
+
+Ltac cannot_crash :=
+  repeat match goal with
+  | H: can_crash |- _ => exfalso; rewrite cannot_crash in H; exact H
+  | H: exec _ _ (Crashed _) |- _ => exfalso; apply exec_cannot_crash in H; exact H
+  | |- rec_noop _ _ _ => apply always_rec_noop
+  end.
